\section{Preliminary Algebra}
\subsection{Coordinate Geometry}
\paragraph{Equation of a line}
$$y = mx + c$$
\paragraph{Equation of a circle}
$${(x-h)}^2 + {(y-k)}^2 = r^2$$
\paragraph{Equation of a parabola}
\begin{align*}
y - k &= a{(x-h)}^2 & x-h = a{(y-k)^2} \\
\end{align*}
\paragraph{Equation of an ellipse}
\begin{align*}
\frac{{(x-h)}^2}{a^2} + \frac{{(y-k)}^2}{b^2} = 1
\end{align*}
\paragraph{Equation of a hyperbola}
\begin{align*}
\frac{{(x-h)}^2}{a^2} - \frac{{(y-k)}^2}{b^2} = 1
\end{align*}


\subsection{Logarithms and Exponentials}
\paragraph{Properties of Exponentials}
\begin{align*}
		&a^n a^m = a^{n+m} & &\frac{a^n}{a^m}   = a^{n-m}\\
		&(a b)^n = a^n  b^n & &\left({\frac{a}{b}}\right)^n  = \frac{a^n}{b^n}\\
		&(a^n)^m = a^{n m} & &\left({\frac{a}{b}}\right)^{-n} = {\frac{b}{a}}^{n}\\
\end{align*}
\paragraph{Properties of Logarithms}
\begin{align*}
&\log_aa  = 1 &   &\log_a1 = 0 \\
&(\log_ab)(\log_bc) = \log_ac & &\log_ab = \frac{1}{\log_ba} \\
&\log_a(xy) = \log_ax + \log_ay &
&\log_a\left(\frac{x}{y}\right) = \log_ax - \log_ay
\end{align*}


\subsection{Binomial Expansion}
$$^nC_k = \frac{n!}{k!(n-k)!} = {n\choose k} $$
Also,
\begin{align*}
	{^nC_0} &= {^nC_n} = 1 \\
	{^nC_1} &= {^nC_{n-1}} = n \\
	{^nC_k} &= {^nC_{n-k}}
\end{align*}
For a binomial expression raised to the power \emph{n}:
$${(x+y)}^n  = \sum_{k=0}^{k=n} {^nC_k} x^{n-k}y^k$$
\paragraph{Pascal's Triangle}
\begin{center}
	~
\vbox{\offinterlineskip
	\halign to 3.2in{\quad\hfil#\hfil\cr
		1 \cr\noalign{\vskip 1 mm}
		1\hskip5.010mm 1 \cr\noalign{\vskip 1 mm}
		1\hskip5.015mm 2\hskip5.015mm 1 \cr\noalign{\vskip 1 mm}
		1\hskip5.025mm 3\hskip5.025mm 3\hskip5.025mm 1 \cr\noalign{\vskip 1 mm}
		1\hskip5.05mm 4\hskip5.05mm 6\hskip5.05mm 4\hskip5.05mm 1 \cr\noalign{\vskip 1.5 mm}
		1\hskip5mm 5\hskip5mm 10\hskip5mm 10\hskip5mm 5\hskip5mm 1 \cr\noalign{\vskip 1.5 mm}
		1\hskip4.90mm 6\hskip4.90mm 15\hskip4.90mm 20\hskip4.90mm 15\hskip4.90mm 6\hskip4.90mm 1 \cr\noalign{\vskip 1.5 mm}
		1\hskip4.75mm 7\hskip4.75mm 21\hskip4.75mm 35\hskip4.75mm 35\hskip4.75mm 21\hskip4.75mm 7\hskip4.75mm 1 \cr\noalign{\vskip 1.5 mm}
		1\hskip4.5mm 8\hskip4.5mm 28\hskip4.5mm 56\hskip4.5mm 70\hskip4.5mm 56\hskip4.5mm 28\hskip4.5mm 8\hskip4.5mm 1 \cr\noalign{\vskip 1.5 mm}
		1\hskip4mm 9\hskip4mm 36\hskip4mm 84\hskip4mm 126\hskip4mm 126\hskip4mm 84\hskip4mm 36\hskip4mm 9\hskip4mm 1 \cr\noalign{\vskip 1.5 mm}
		1\hskip3mm 10\hskip3mm 45\hskip3mm 120\hskip3mm 210\hskip3mm 252\hskip3mm 210\hskip3mm 120\hskip3mm 45\hskip3mm 10\hskip3mm 1 \cr\noalign{\vskip 1.5 mm}
	}
}
\end{center}
\paragraph{Commonly Factored Polynomials}

$$
\begin{array}{lcl}
		{x^2-y^2} &=& (x-y)(x+y) \\
		{(x+y)^2} &=& x^2+2xy+y^2\\
		{(x-y)^2} &=& x^2-2xy+y^2\\
		{x^3-y^3} &=& (x-y)(x^2+xy+y^2)\\
		{x^3+y^3} &=& (x+y)(x^2-xy+y^2)\\
		{(x+y)^3} &=& x^3+3x^2y+3xy^2+y^3\\
		{(x-y)^3} &=& x^3-3x^2y+3xy^2-y^3\\
\end{array}
$$


